# Copyright (c) 2021 Iotic Labs Ltd. All rights reserved.

###############################################################################
# IOTICS Resource Ontology                                                    #
###############################################################################

PREFIX rdf:     <http://www.w3.org/1999/02/22-rdf-syntax-ns#>
PREFIX rdfs:    <http://www.w3.org/2000/01/rdf-schema#>
PREFIX xsd:     <http://www.w3.org/2001/XMLSchema#>

PREFIX iotics:    <http://data.iotics.com/iotics#>

## Base ontology for IOTICS Digital Twins and the data they share.

iotics:DigitalTwin
    a rdfs:Class ;
    rdfs:label "IOTICS Digital Twin"@en ;
    rdfs:comment "A virtual representation of a real asset, device, concept or person in an IOTICSpace"@en ;
    .

iotics:HostTwin
    a rdfs:Class ;
    rdfs:subClassOf iotics:DigitalTwin ;
    rdfs:label "IOTICS Host Twin"@en ;
    rdfs:comment "The Digital Twin of an IOTICS Host"@en ;
    .

iotics:advertises
    a rdf:Property ;
    rdfs:label "Advertises"@en ;
    rdfs:comment "This property lists (advertises) what mechanisms (points) the Digital Twin has to interact with other Twins"@en ;
    rdfs:domain iotics:DigitalTwin ;
    rdfs:range iotics:Point ;
    .

iotics:Visibility
    a rdfs:Class ;
    rdfs:label "Visibility"@en ;
    rdfs:comment "Defines whether an IOTICS Digital Twin may be found or described from other Hosts"@en ;
    .

iotics:public
    a iotics:Visibility ;
    rdfs:label "Public"@en ;
    rdfs:comment "A public Digital Twin can be found or described from other Hosts"@en ;
    .

iotics:private
    a iotics:Visibility ;
    rdfs:label "Private"@en ;
    rdfs:comment "A private Digital Twin can only be found or described from the local Host"@en ;
    .

iotics:hasVisibility
    a rdf:Property ;
    rdfs:comment "Property relating an IOTICS Digital Twin to a certain Visibility level"@en ;
    rdfs:domain iotics:DigitalTwin ;
    rdfs:range  iotics:Visibility ;
    .

iotics:Point
    a rdfs:Class ;
    rdfs:label "IOTICS Point"@en ;
    rdfs:comment """A means by which an IOTICS Digital Twin may interact with other twins, either outbound or inbound.
        Metadata describing the payload of the point is available when the point is described and therefore separate to the
        payload data. Interactions with the point are brokered and secured according to policies controlled by the twin."""@en ;
    .

iotics:pointName
    # we need to capture here the restructions:
    # - a twin can't have two different feeds with the same pointName
    # - a feed can't have two or more  pointName properties
	a rdf:Property ;
    rdfs:label "IOTICS Point name"@en ;
    rdfs:comment "The name of the point. This must be unique per Digital Twin."@en ;
	rdfs:domain iotics:Point ;
	rdfs:range xsd:string ;
	.

iotics:Feed
    a rdfs:Class ;
    rdfs:subClassOf iotics:Point ;
    rdfs:label "IOTICS Data Feed"@en ;
    rdfs:comment """A feed of data advertised by an IOTICS Digital Twin, used by the twin to broadcast values.
        Authorised twins following this feed receive data when published"""@en ;
    .

iotics:storesLast
    a rdf:Property ;
    rdfs:label "Stores last published payload"@en ;
    rdfs:comment "Whether most recent published payload might be available on this feed."@en ;
    rdfs:domain iotics:Feed ;
    rdfs:range xsd:boolean ;
    .

iotics:Input
    a rdfs:Class ;
    rdfs:subClassOf iotics:Point ;
    rdfs:label "IOTICS Input"@en ;
    rdfs:comment """By advertising an input, an IOTICS Digital Twin allows authorised twins to send messages whose meaning
    might be described by the properties of the input itself and of its payload.
    For example, inputs can be used to send commands to change the state of the underlying asset or to send messages
    that can be interpreted by the twin to implement request/response exchanges."""@en ;
    .

iotics:Value
    a rdfs:Class ;
    rdfs:label "IOTICS Payload Value"@en ;
    rdfs:comment "A semantic description of a Value used by Points when communicating data"@en ;
    .

iotics:valueKey
    a rdf:Property ;
    rdfs:subPropertyOf rdfs:label ;
    rdfs:label "Value Key"@en ;
    rdfs:comment "Unique identifier for this Value among those offered by its Point."@en ;
    rdfs:domain iotics:Value ;
    .

iotics:valueType
    a rdf:Property ;
    rdfs:label "Value Type"@en ;
    rdfs:comment "The xsd datatype of the Value, e.g. xsd:decimal. See https://www.w3.org/TR/rdf11-concepts/#xsd-datatypes"@en ;
    rdfs:domain iotics:Value ;
    # is there a way to restrct the range to some ontology that captures the xsd data types?
    .

iotics:valueUnit
    a rdf:Property ;
    rdfs:label "Value Unit"@en ;
    rdfs:comment "The unit of the value, e.g. obo:UO_0000027 representing Celsius degrees"@en ;
    rdfs:domain iotics:Value ;
    .

iotics:presents
    a rdf:Property ;
    rdfs:label "Presents"@en ;
    rdfs:comment """The property defining what values compose the payload of this point. For example, a feed for a weather station
        may have a payload with two values representing temperature and pressure defined as iotics:Value resources."""@en ;
    rdfs:domain iotics:Point ;
    rdfs:range iotics:Value ;
    .

iotics:hasEndpoint
    a rdf:Property ;
    rdfs:label "has Endpoint"@en ;
    rdfs:comment "Relates twins to their endpoints"@en ;
    rdfs:domain iotics:Twin ;
    rdfs:range iotics:Endpoint ;
    .

iotics:Endpoint
    a rdfs:Class ;
    rdfs:label "Endpoint"@en ;
    rdfs:comment "A means of interacting with a Twin"@en ;
    .

iotics:ApiEndpoint
    a rdfs:Class;
    rdfs:subClassOf iotics:Endpoint;
    .

iotics:NetworkEndpoint
    a rdfs:Class ;
    rdfs:subClassOf iotics:Endpoint ;
    .

iotics:allows
    a rdf:Property ;
    rdfs:label "Allows"@en ;
    rdfs:comment "Relates endpoints to the identities allowed to access them"@en ;
    rdfs:domain iotics:Endpoint ;
    # range handled via SHACL
    .

iotics:AllowListValue
    a rdfs:Class ;
    rdfs:label "Allow list value"@en ;
    rdfs:comment "Values indicating that all or no resources are allowed access via the network or API"@en ;
    .

iotics:allowAll
    a iotics:AllowListValue ;
    rdfs:label "Allow All"@en ;
    .

iotics:allowNone
    a iotics:AllowListValue ;
    rdfs:label "Allow None"@en ;
    .

iotics:User
    # Taken from Tim's concepts document, since this is now used in the ApiAllowListShape. What else can we say about it?
    rdf:type rdfs:Class ;
    rdfs:label "User"@en ;
    rdfs:comment "An Identity of type User"@en ;
    .
