PREFIX rdf:     <http://www.w3.org/1999/02/22-rdf-syntax-ns#>
PREFIX rdfs:    <http://www.w3.org/2000/01/rdf-schema#>
PREFIX xsd:     <http://www.w3.org/2001/XMLSchema#>

PREFIX iotics:  <http://data.iotics.com/iotics#>
PREFIX pub:     <http://data.iotics.com/public#>

pub:HostTwin
    rdf:type rdfs:Class ;
    rdfs:subClassOf pub:AllowListValue ;
    rdfs:subClassOf iotics:DigitalTwin ;
    rdfs:label "Iotics Host Twin"@en ;
    rdfs:comment "The Iotics Host virtual counterpart"@en ;
    .

pub:hostAllowList
    rdf:type rdf:Property ;
    rdfs:label "Host Data allow list"@en ;
    rdfs:comment "Determines whether a Digital Twin's Data is accessible or not by a Digital Twin from other Hosts. The Twin's Data will always be accessible to other Twins in the same Host."@en ;
    rdfs:domain iotics:DigitalTwin ;
    rdfs:range pub:AllowListValue ;
    .

pub:hostMetadataAllowList
    rdf:type rdf:Property ;
    rdfs:label "Host Metadata allow list"@en ;
    rdfs:comment "Determines whether the Digital Twin's Metadata is visible or not to other Hosts. The Twin's Metadata will always be visible in the same Host"@en ;
    rdfs:domain iotics:DigitalTwin ;
    rdfs:range pub:AllowListValue ;
    .

pub:AllowListValue rdf:type rdfs:Class ;
    rdfs:label "Allow list value"@en ;
    rdfs:comment "Host network allow list value"@en ;
.

pub:allHosts
    rdf:type pub:AllowListValue ;
    rdfs:label "Allow all hosts value"@en ;
    rdfs:comment "Allow list value used to allow interactions initiated from any remote host to the resource over the network"@en ;
    .

pub:noHost
    rdf:type iotics:AllowListValue ;
    rdfs:label "No host allowed value"@en ;
    rdfs:comment "Allow list Value used to deny any interaction initiated from a remote host to the resource over the network"@en ;
    .
