# Copyright (c) 2021 Iotic Labs Ltd. All rights reserved.

###############################################################################
# IOTIC Public Ontology                                                       #
###############################################################################

PREFIX iotb:    <http://purl.org/net/iotic-labs#>
PREFIX pub:     <http://data.iotics.com/public#>
PREFIX rdf:     <http://www.w3.org/1999/02/22-rdf-syntax-ns#>
PREFIX rdfs:    <http://www.w3.org/2000/01/rdf-schema#>
PREFIX xsd:     <http://www.w3.org/2001/XMLSchema#>

pub:HostTwin
    rdf:type rdfs:Class ;
    rdfs:subClassOf pub:AllowListValue ;
    rdfs:label "Iotics Host Twin"@en ;
    rdfs:comment "The Iotics Host virtual counterpart"@en ;
    .

pub:apiAllowList
    rdf:type rdf:Property ;
    rdfs:label "API allow list"@en ;
    rdfs:comment "User or Twin DIDs allowed to interact with the host API"@en ;
    rdfs:domain pub:HostTwin;
    rdfs:range xsd:string ;
    .

pub:hostAllowList
    rdf:type rdf:Property ;
    rdfs:label "Host network allow list"@en ;
    rdfs:comment "Host twin DIDs (or allow all/none predefined allowed values) allowed to interact with the resource over the network"@en ;
    rdfs:domain iotb:Entity;
    rdfs:range pub:AllowListValue ;
    .

pub:AllowListValue rdf:type rdfs:Class ;
    rdfs:label "Allow list value"@en ;
    rdfs:comment "Host network allow list value"@en ;
.

pub:allHosts
    rdf:type pub:AllowListValue ;
    rdfs:label "Allow all hosts value"@en ;
    rdfs:comment "Allow list value used to allow interactions initiated from any remote host to the resource over the network"@en ;
    .

pub:noHost
    rdf:type pub:AllowListValue ;
    rdfs:label "No host allowed value"@en ;
    rdfs:comment "Allow list Value used to deny any interaction initiated from a remote host to the resource over the network"@en ;
    .
