@prefix iotics: <http://localhost:8000/> .
@prefix rdfs: <http://www.w3.org/2000/01/rdf-schema#> .

iotics:hostAllowList
    rdf:type rdf:Property ;
    rdfs:label "Host Data allow list"@en ;
    rdfs:comment "Determines whether a Digital Twin's Data is accessible or not by a Digital Twin from other Hosts. The Twin's Data will always be accessible to other Twins in the same Host."@en ;
    rdfs:domain iotics:DigitalTwin ;
    rdfs:range iotics:AllowListValue ;
    .

iotics:hostMetadataAllowList
    rdf:type rdf:Property ;
    rdfs:label "Host Metadata allow list"@en ;
    rdfs:comment "Determines whether the Digital Twin's Metadata is visible or not to other Hosts. The Twin's Metadata will always be visible in the same Host."@en ;
    rdfs:domain iotics:DigitalTwin ;
    rdfs:range iotics:AllowListValue ;
    .

iotics:userAllowList
    rdf:type rdf:Property ;
    rdfs:label "User allow list"@en ;
    rdfs:comment "Determines whether a set of user identities are allowed to perform an action against the Iotics API."@en ;
    rdfs:domain iotics:DigitalTwin ;
    rdfs:range iotics:AllowListValue ;
    .

iotics:agentAllowList
    rdf:type rdf:Property ;
    rdfs:label "Agent allow list"@en ;
    rdfs:comment "Determines whether a set of agent identities are allowed to perform an action against the Iotics API."@en ;
    rdfs:domain iotics:DigitalTwin ;
    rdfs:range iotics:AllowListValue ;
    .

iotics:AllowListValue rdf:type rdfs:Class ;
    rdfs:label "Allow list value"@en ;
    rdfs:comment "Value expected to be a DID or one of iotics:all or iotics:none."@en ;
.

iotics:all
    rdf:type iotics:AllowListValue ;
    rdfs:label "All identities allowed value"@en ;
    rdfs:comment "Allow list value used to allow any interaction initiated by the related identity."@en ;
    .

iotics:none
    rdf:type iotics:AllowListValue ;
    rdfs:label "No identities allowed value"@en ;
    rdfs:comment "Allow list value used to deny any interaction initiated by the related identity."@en ;
    .
