@prefix iotics: <http://localhost:8000/> .
@prefix dcterms: <http://purl.org/dc/terms/> .
@prefix vann: <http://purl.org/vocab/vann/> .
@prefix foaf: <http://xmlns.com/foaf/0.1/> .
@prefix owl: <http://www.w3.org/2002/07/owl#> .
@prefix rdf: <http://www.w3.org/1999/02/22-rdf-syntax-ns#> .
@prefix xml: <http://www.w3.org/XML/1998/namespace> .
@prefix xsd: <http://www.w3.org/2001/XMLSchema#> .
@prefix rdfs: <http://www.w3.org/2000/01/rdf-schema#> .

iotics:Asset
    a rdfs:Class ;
    rdfs:label "Asset"@en ;
    rdfs:comment """A 'real' asset (person, device, system, algorithm, etc.) that can be virtualised. 
An asset may be the combination of multiple 'real' objects. This classifier is kept purposefully generic.
"""@en ;
    .

iotics:virtualises
    a rdf:Property ;
    rdfs:label "virtualises"@en ;
    rdfs:comment "Links an asset with its own digital twin."@en ;
    rdfs:domain iotics:DigitalTwin ;
    rdfs:range iotics:Asset ;
    .

iotics:DigitalTwin
    a rdfs:Class ;
    rdfs:label "IOTICS Digital Twin"@en ;
    rdfs:comment "A virtual representation of a real asset, device, concept or person in an IOTICSpace"@en ;
    .

## we need a shape saying that HostTwin virtualise a Host
iotics:HostTwin
    a rdfs:Class ;
    rdfs:subClassOf iotics:DigitalTwin ;
    rdfs:label "Host Twin"@en ;
    rdfs:comment "The Digital Twin of an IOTICS Host"@en ;
    iotics:virtualises iotics:Host ;
    .

iotics:advertises
    a rdf:Property ;
    rdfs:label "advertises"@en ;
    rdfs:comment "Lists (advertises) what mechanisms (points) the Digital Twin has to interact with other Twins"@en ;
    rdfs:domain iotics:DigitalTwin ;
    rdfs:range iotics:Point ;
    .

iotics:createdAt
    a rdf:Property ;
    rdfs:label "created at"@en ;
    rdfs:comment "The date on which a IOTICS Digital Twin was created"@en ;
    rdfs:domain iotics:DigitalTwin ;
    rdfs:range xsd:dateTime
    .

iotics:updatedAt
    a rdf:Property ;
    rdfs:label "updated at"@en ;
    rdfs:comment """The date on which an IOTICS Digital Twin,
or any of its feeds or inputs was updated, including updates which 
do not otherwise modify the Digital Twin, its feeds or inputs
"""@en ;
    rdfs:domain iotics:DigitalTwin ;
    rdfs:range xsd:dateTime ;
    .

iotics:Point
    a rdfs:Class ;
    rdfs:label "Twin Point"@en ;
    rdfs:comment """A means by which an IOTICS Digital Twin may interact with other twins, either outbound or inbound.
Metadata describing the payload of the point is available when the point is described and therefore separate to the
payload data. Interactions with the point are brokered and secured according to policies controlled by the twin.
"""@en ;
    .

iotics:pointName
    # we need to capture here the restructions:
    # - a twin can't have two different feeds with the same pointName
    # - a feed can't have two or more  pointName properties
	a rdf:Property ;
    rdfs:label "point name"@en ;
    rdfs:comment "The name of the point. This must be unique per type of point for a given Digital Twin."@en ;
	rdfs:domain iotics:Point ;
	rdfs:range xsd:string ;
	.

iotics:Feed
    a rdfs:Class ;
    rdfs:subClassOf iotics:Point ;
    rdfs:label "Twin Feed"@en ;
    rdfs:comment """A feed of data advertised by an IOTICS Digital Twin, used by the twin to broadcast values.
Authorised twins following this feed receive data when published"""@en ;
    .

iotics:storesLast
    a rdf:Property ;
    rdfs:label "stores last"@en ;
    rdfs:comment "Stores last published payload: whether most recent published payload might be available on this feed."@en ;
    rdfs:domain iotics:Feed ;
    rdfs:range xsd:boolean ;
    .

iotics:Input
    a rdfs:Class ;
    rdfs:subClassOf iotics:Point ;
    rdfs:label "Twin Input"@en ;
    rdfs:comment """By advertising an input, an IOTICS Digital Twin allows authorised twins to send messages whose meaning
might be described by the properties of the input itself and of its payload.
For example, inputs can be used to send commands to change the state of the underlying asset or to send messages
that can be interpreted by the twin to implement request/response exchanges.
"""@en ;
    .

iotics:Value
    a rdfs:Class ;
    rdfs:label "Point Payload Value"@en ;
    rdfs:comment "A semantic description of a Value used by Points when communicating data"@en ;
    .

iotics:valueKey
    a rdf:Property ;
    rdfs:subPropertyOf rdfs:label ;
    rdfs:label "value key"@en ;
    rdfs:comment "Unique identifier for this Value among those offered by its Point."@en ;
    rdfs:domain iotics:Value ;
    rdfs:range xsd:string ;
    .

iotics:valueType
    a rdf:Property ;
    rdfs:label "value type"@en ;
    rdfs:comment "The xsd datatype of the Value, e.g. xsd:decimal. See https://www.w3.org/TR/rdf11-concepts/#xsd-datatypes"@en ;
    rdfs:domain iotics:Value ;
    # is there a way to restrct the range to some ontology that captures the xsd data types?
    .

iotics:valueUnit
    a rdf:Property ;
    rdfs:label "value unit"@en ;
    rdfs:comment "The unit of the value, e.g. obo:UO_0000027 representing Celsius degrees"@en ;
    rdfs:domain iotics:Value ;
    .

iotics:presents
    a rdf:Property ;
    rdfs:label "presents"@en ;
    rdfs:comment """The property defining what values compose the payload of this point. For example, a feed for a weather station
may have a payload with two values representing temperature and pressure defined as iotics:Value resources.
"""@en ;
    rdfs:domain iotics:Point ;
    rdfs:range iotics:Value ;
    .

