@prefix iotics: <http://localhost:8000/> .
@prefix org: <http://www.w3.org/ns/org#> .
@prefix foaf: <http://xmlns.com/foaf/0.1/> .
@prefix owl: <http://www.w3.org/2002/07/owl#> .
@prefix rdf: <http://www.w3.org/1999/02/22-rdf-syntax-ns#> .
@prefix xsd: <http://www.w3.org/2001/XMLSchema#> .
@prefix rdfs: <http://www.w3.org/2000/01/rdf-schema#> .

iotics:Participant
    a rdfs:Class;
    rdfs:subClassOf foaf:Agent, org:Organization;
    rdfs:label "Participant"@en;
    rdfs:comment "Stakeholder owning a component in IOTICS or managed by IOTICS."@en;
    .

iotics:InfrastructureComponent 
    a rdfs:Class;
    rdfs:label "InfrastructureComponent"@en ;
    rdfs:comment """The class of all infrastructure components in IOTICS. 
Anything that is part of the physical infrastructure of the IOTICS offering can use this classifier.
"""@en;
    .

iotics:ConfigurationParameter
    a rdfs:Class;
    rdfs:label "ConfigurationParameter"@en ;
    rdfs:comment """The class of all configuration parameters for IOTICSpace and components."""@en;
    .

iotics:hasCommonName
	a rdf:Property ;
	rdfs:label "common name"@en;
	rdfs:comment "Commonly used name or term for the Participant."@en ;
	rdfs:domain iotics:Participant ;
	rdfs:range xsd:string ;
	.

iotics:hasLegalName
	a rdf:Property ;
	rdfs:label "legal name"@en;
	rdfs:comment """The complete legal name of a Participant. 
Unlike the name the participant which refers to the commonly used name 
or term for the Participant, a legal name identifies a participant for legal, 
administrative and other official purposes."""@en ;
	rdfs:domain iotics:Participant ;
	rdfs:range xsd:string ;
	.

iotics:maintainer 
    a rdf:Property;
    rdfs:label "maintainer"@en;
    rdfs:comment "Participant responsible for technical maintenance of the InfrastructureComponent."@en ;
    rdfs:domain iotics:InfrastructureComponent;
    rdfs:range iotics:Participant;
    .

iotics:componentVersion 
	a rdf:Property ;
    rdfs:label "component version"@en;
    rdfs:comment "InfrastructureComponent version."@en ;
    rdfs:domain iotics:InfrastructureComponent;
    rdfs:range xsd:string;
    .

iotics:Connector
    rdfs:subClassOf iotics:InfrastructureComponent ;
    a rdfs:Class ;
    rdfs:comment """A connector is an Agent application that typically manages the creation and behaviour 
of multiple twins. Typically connectors act on behalf of a single non-human user, and their execution is automated.
Connectors are multi-tenanted as far as twins are concerned and single-tenanted as far as users are concerned.
A connector needs a runtime environment to run, outside IOTICS.
It's uncommon but a connector can implement more than one agent concurrently depending on the user requirements. For example a simulator of
multiple real agents that are bundled in a single application.
"""@en ;
    rdfs:label "Connector"@en 
    .


iotics:Host
    rdfs:subClassOf iotics:InfrastructureComponent ;
    a rdfs:Class, iotics:Asset ;
    rdfs:label "Host" ;
    rdfs:comment """The host is a server providing access to Twin's metadata and provides the necessary 
infrastructure for twins to publish/subscribe data and send/receive inputs.
Host provides an API endpoint for agents to interact with the 'local' twins and with twins in remote hosts.
Metadata is stored in a triple store database in the host.
One or more hosts are deployed in an IOTICSpace""" ;
 .

iotics:CentralisedResolverSystem
    rdfs:subClassOf iotics:InfrastructureComponent, iotics:Resolver;
    a rdfs:Class ;
    rdfs:label "Centralised Resolver System" ;
    rdfs:comment "This is a Centralised Resolver that is hosted by IOTICS to provide resolver capabilities for IOTICSpaces hosted by IOTICS" ;
 .

iotics:IoticSpace
    a iotics:Asset ;
    rdfs:label "IOTICSpace" ;
    rdfs:comment "An IOTICSpace is IOTICS product." ;
 .

 iotics:groups 
    a rdf:Property;
    rdfs:label "groups"@en;
    rdfs:comment "An IOTICSpace is a logical grouping of a set of distinct infrastructure components and configuration parameters"@en ;
    rdfs:domain iotics:IoticSpace;
    rdfs:range [ rdf:type rdfs:Class ;
                owl:unionOf ( iotics:InfrastructureComponent iotics:ConfigurationParameter)
              ] ;
    .

iotics:IoticsUI
    rdfs:subClassOf iotics:InfrastructureComponent ;
    a rdfs:Class ;
    rdfs:label "IOTICS UI" ;
    rdfs:comment "IOTICS UI is a browser based application allowing to interact with IOTICSpace" ;
 .

iotics:Network
    a rdfs:Class ;
    rdfs:label "Netowrk" ;
    rdfs:comment "A netowrk is a set of hosts connected to each other and able to exchange data with each other" ;
 .

iotics:connects 
    a rdf:Property;
    rdfs:label "connects"@en;
    rdfs:comment "A network connects multiple hosts"@en ;
    rdfs:domain iotics:Network;
    rdfs:range iotics:Host;
    .

iotics:trafficEncryptedBy
    a rdf:Property;
    rdfs:label "traffic enchrypted by"@en;
    rdfs:comment "Network traffic for this host is enchrypted by a pnet key"@en ;
    rdfs:domain iotics:Host;
    rdfs:range iotics:PnetKey;
    .

iotics:hasEndpoint
    a rdf:Property ;
    rdfs:label "has endpoint"@en ;
    rdfs:comment "Relates twins to their endpoints"@en ;
    rdfs:domain iotics:Twin ;
    rdfs:range iotics:Endpoint ;
    .

iotics:Endpoint
    a rdfs:Class ;
    rdfs:label "Endpoint"@en ;
    rdfs:comment "A means of interacting with a twin or host"@en ;
    .

iotics:grpcEndpoint
    a iotics:IoticsAgentAPI ;
    rdfs:label "gRPC Endpoint"@en ;
    rdfs:comment "A means of interacting with a twin or host via gRPC"@en ;
    .

iotics:restStompEndpoint
    a iotics:IoticsAgentAPI ;
    rdfs:label "REST/STOMP Endpoint"@en ;
    rdfs:comment "A means of interacting with a twin or host via REST and STOMP/Websocket"@en ;
    .

iotics:IoticsNetworkAPI
    a iotics:Endpoint ;
    rdfs:label "IOTICS network api" ;
    rdfs:comment "The API used by hosts to communicate with each other" ;
 .

iotics:IoticsAgentAPI
    rdfs:subClassOf iotics:Endpoint ;
    a rdfs:Class ;
    rdfs:label "IOTICS agent api" ;
    rdfs:comment "The API used by agents to interact with a Host. This API is private in the sense that it is accessible only by the owner of the Host." ;
 .


iotics:IoticsResolverAPI
    rdfs:subClassOf iotics:Endpoint ;
    a rdfs:Class ;
    rdfs:label "IOTICS resolver api" ;
    rdfs:comment """The API used by the Resolver System. 
This API allows clients to store or retrieve DID Documents by their DID. 
It is also used by Hosts to verify delegations for any incoming requests.""" ;
 .

iotics:ClientArtifact
    a rdfs:Class ;
    rdfs:subClassOf iotics:InfrastructureComponent ;
    rdfs:label "IOTICS client library" ;
    rdfs:comment "Any software component/library provided by IOTICS that can be used to build applications (agents, connectors) that interact with IOTICS" ;
    .

iotics:isSupported
    a rdf:Property ;
    rdfs:label "is supported" ;
    rdfs:comment "if true the library is supported by IOTICS" ;
    rdfs:domain iotics:ClientArtifact ;
    rdfs:range xsd:boolean ;
    .

iotics:forLanguage
    a rdf:Property ;
    rdfs:label "for language" ;
    rdfs:comment "the language/environment this library is for" ;
    rdfs:domain iotics:ClientArtifact ;
    rdfs:range xsd:string ;
    .

iotics:IdentityLibrary
    a rdfs:Class ;
    rdfs:subClassOf iotics:ClientArtifact ;
    rdfs:label "IOTICS Identity Library" ;
    rdfs:comment "Client software library implementing the IOTICS DID specification." ;
    .

iotics:goIdentityLibrary
    a iotics:IdentityLibrary ;
    rdfs:label "GOLANG Identity Library" ;
    iotics:isSupported true ;
    iotics:forLanguage "golang" ;
    .

iotics:pythonIdentityLibrary
    a iotics:IdentityLibrary ;
    rdfs:label "PYTHON Identity Library" ;
    iotics:isSupported true ;
    iotics:forLanguage "python" ;
    .

iotics:rustIdentityLibrary
    a iotics:IdentityLibrary ;
    rdfs:label "RUST Identity Library" ;
    iotics:isSupported true ;
    iotics:forLanguage "rust" ;
    .

iotics:ApiLibrary
    a rdfs:Class ;
    rdfs:subClassOf iotics:ClientArtifact ;
    rdfs:label "IOTICS API Library" ;
    rdfs:comment "Client software library implementing the IOTICS API for agents/connectors to interact with IOTICSpace hosts." ;
    .

iotics:integratesEndpoint
    a rdf:Property ;
    rdfs:label "integrates endpoint" ;
    rdfs:comment "What endpoint this API library integrates with." ;
    rdfs:domain iotics:ApiLibrary ;
    rdfs:range iotics:Endpoint ;
    .

iotics:stompApiLibrary
    a iotics:ApiLibrary ;
    rdfs:label "STOMP API Library" ;
    iotics:isSupported true ;
    iotics:forLanguage "python" ;
    iotics:integratesEndpoint iotics:restStompEndpoint ;
    .

iotics:javaApiLibrary
    a iotics:ApiLibrary ;
    rdfs:label "JAVA API Library" ;
    iotics:isSupported false ;
    iotics:forLanguage "java" ;
    iotics:integratesEndpoint iotics:grpcEndpoint ;
    .

iotics:typescriptApiLibrary
    a iotics:IdentityLibrary ;
    rdfs:label "TYPESCRIPT API Library" ;
    iotics:isSupported true ;
    iotics:forLanguage "typescript" ;
    iotics:integratesEndpoint iotics:grpcEndpoint ;
    .

iotics:pythonApiLibrary
    a iotics:IdentityLibrary ;
    rdfs:label "PYTHON API Library" ;
    iotics:isSupported true ;
    iotics:forLanguage "python" ;
    iotics:integratesEndpoint iotics:grpcEndpoint ;
    .

iotics:rustApiLibrary
    a iotics:IdentityLibrary ;
    rdfs:label "RUST API Library" ;
    iotics:isSupported true ;
    iotics:forLanguage "rust" ;
    iotics:integratesEndpoint iotics:grpcEndpoint ;
    .
